hol/equationScript.sml
@@ -1,0 +1,89 @@
+open HolKernel boolLib bossLib Parse SatisfySimps termTheory substitutionTheory pred_setTheory pairTheory finite_mapTheory lcsymtacs
+
+val _ = new_theory "equation"
+
+val _ = type_abbrev("equation", ``:('a,'b) term # ('a,'b) term``);
+
+val SAPPLYeq_def = Define`
+  SAPPLYeq s (t1,t2) = (SAPPLY s t1, SAPPLY s t2)`;
+val _ = export_rewrites ["SAPPLYeq_def"];
+
+val set_unifier_def = Define`
+  set_unifier eqs = {s | ∀t1 t2. (t1,t2) ∈ eqs ⇒ (SAPPLY s t1 = SAPPLY s t2)}`;
+
+val varseq_def = Define`
+  varseq (t1, t2) = vars t1 ∪ vars t2`;
+val _ = export_rewrites ["varseq_def"];
+
+val FINITE_varseq = Q.store_thm(
+"FINITE_varseq",
+`FINITE (varseq eq)`,
+Cases_on `eq` >> srw_tac [][]);
+val _ = export_rewrites ["FINITE_varseq"];
+
+val solved_form_def = Define`
+  solved_form eqs =
+    FINITE eqs ∧
+    ∀eq. eq ∈ eqs ⇒
+         ∃v t. (eq = (Var v, t)) ∧ (v ∉ vars t) ∧
+               ∀eq'. eq' ∈ eqs ∧ eq' ≠ eq ⇒ v ∉ varseq eq'`;
+
+val eqsvdom_def = Define`eqsvdom eqs = {v | ∃t. (Var v, t) ∈ eqs}`
+
+val FINITE_eqsvdom = store_thm(
+  "FINITE_eqsvdom",
+  ``FINITE eqs ⇒ FINITE (eqsvdom eqs)``,
+  strip_tac >>
+  `eqsvdom eqs ⊆ (IMAGE (term_case I ARB o FST) eqs)` by (
+    srw_tac [][SUBSET_DEF,eqsvdom_def] >- (
+    qexists_tac `(Var x, t)` >> srw_tac [][] ) >>
+  full_simp_tac (srw_ss()) [solved_form_def] >>
+  res_tac >> srw_tac [][] >>
+  qexists_tac `t` >> asm_simp_tac pure_ss [] ) >>
+  metis_tac [SUBSET_FINITE, IMAGE_FINITE]);
+
+val solved_form_functional = store_thm(
+  "solved_form_functional",
+  ``solved_form eqs ∧ (v,t1) ∈ eqs ∧ (v,t2) ∈ eqs ⇒ (t1 = t2)``,
+  srw_tac [][solved_form_def] >>
+  first_x_assum (Q.SPEC_THEN `(v,t1)` MP_TAC) >>
+  asm_simp_tac (srw_ss()) [] >>
+  DISCH_THEN (Q.X_CHOOSE_THEN `w` STRIP_ASSUME_TAC) >>
+  first_x_assum (Q.SPEC_THEN `(v,t2)` MP_TAC) >>
+  asm_simp_tac (srw_ss()) []);
+
+val solved_form_unifier = Q.store_thm(
+"solved_form_unifier",
+`solved_form eqs ⇒
+   (FUN_FMAP (λv. @t. (Var v,t) ∈ eqs) (eqsvdom eqs)) ∈ set_unifier eqs`,
+strip_tac >>
+Q.MATCH_ABBREV_TAC `FUN_FMAP f P ∈ set_unifier eqs` >>
+`FINITE eqs` by full_simp_tac pure_ss [solved_form_def] >>
+`FINITE P` by metis_tac [FINITE_eqsvdom] >>
+srw_tac [][set_unifier_def] >>
+`∃v. t1 = Var v` by metis_tac [solved_form_def, PAIR_EQ] >>
+`v ∈ P` by srw_tac [SATISFY_ss][Abbr`P`,eqsvdom_def] >>
+srw_tac [][FLOOKUP_FUN_FMAP] >>
+`f v = t2` by (srw_tac [][Abbr`f`] >> SELECT_ELIM_TAC >>
+               metis_tac [solved_form_functional]) >>
+qsuff_tac `DISJOINT (FDOM (FUN_FMAP f P)) (vars t2)`
+  >- metis_tac [FDOM_DISJOINT_vars] >>
+asm_simp_tac (srw_ss())[FUN_FMAP_DEF, DISJOINT_DEF, EXTENSION] >>
+qx_gen_tac `w` >> Cases_on `w ∈ P` >> asm_simp_tac (srw_ss()) [] >>
+`∃t. (Var w,t) ∈ eqs`
+  by full_simp_tac (srw_ss() ++ SATISFY_ss)
+                   [Abbr`P`, eqsvdom_def] >>
+`v ∉ vars t2` by metis_tac [solved_form_def, PAIR_EQ, term_11] >>
+full_simp_tac (srw_ss()) [solved_form_def] >>
+first_x_assum (Q.SPEC_THEN `(Var w,t)` MP_TAC) >>
+srw_tac [][] >>
+first_x_assum (Q.SPEC_THEN `(Var v,f v)` MP_TAC) >>
+srw_tac [][] >> metis_tac []);
+
+(* prove the solved form unifier most general? *)
+
+val fsym_counteq_def = Define`
+  fsym_counteq (t1, t2) = fsym_count t1 + fsym_count t2`;
+val _ = export_rewrites ["fsym_counteq_def"];
+
+val _ = export_theory ()
