hol/substitutionScript.sml
@@ -1,0 +1,74 @@
+open HolKernel boolLib bossLib Parse termTheory finite_mapTheory listTheory relationTheory pred_setTheory lcsymtacs
+
+val _ = new_theory "substitution";
+
+val _ = type_abbrev("substitution", ``:'a |-> ('a,'b) term``);
+
+(*val SAPPLY_def = Define*)
+val SAPPLY_def = TotalDefn.tDefine "SAPPLY"`
+  (SAPPLY s (Var v) = case FLOOKUP s v of SOME t -> t || NONE -> (Var v)) ∧
+  (SAPPLY s (App f xs) = App f (MAP (SAPPLY s) xs))`
+( WF_REL_TAC `measure (term_size ARB ARB o SND)` >>
+  metis_tac [subterms_smaller,prim_recTheory.measure_thm,term_size_def] );
+val _ = export_rewrites ["SAPPLY_def"];
+
+val psubterm_mono_SAPPLY = Q.store_thm(
+"psubterm_mono_SAPPLY",
+`∀t u. psubterm t u ⇒ psubterm (SAPPLY s t) (SAPPLY s u)`,
+gen_tac >> ho_match_mp_tac psubterm_ind >>
+srw_tac [][psubterm_cases,MEM_MAP] >>
+metis_tac []);
+
+val TC_psubterm_mono_SAPPLY = save_thm(
+"TC_psubterm_mono_SAPPLY",
+TC_lifts_monotonicities |>
+Q.GEN `f` |> Q.ISPEC `SAPPLY s` |>
+Q.GEN `R` |> Q.ISPEC `psubterm` |>
+C MATCH_MP psubterm_mono_SAPPLY);
+
+val rangevars_def = Define`
+  rangevars s = BIGUNION (IMAGE vars (FRANGE s))`;
+
+val FDOM_DISJOINT_vars = Q.store_thm(
+"FDOM_DISJOINT_vars",
+`DISJOINT (FDOM s) (vars t) ⇒ (SAPPLY s t = t)`,
+Q.ID_SPEC_TAC `t` >>
+ho_match_mp_tac term_ind >>
+srw_tac [][IN_DISJOINT,FLOOKUP_DEF] >>
+full_simp_tac (srw_ss()) [MEM_MAP,EVERY_MEM,MEM_EL,LIST_EQ_REWRITE] >>
+srw_tac [][rich_listTheory.EL_MAP] >>
+metis_tac []);
+
+val NOTIN_rangevars_IN_vars = Q.store_thm(
+"NOTIN_rangevars_IN_vars",
+`!t v s. v IN vars (SAPPLY s t) /\ v NOTIN rangevars s ==> v IN vars t`,
+ho_match_mp_tac term_ind >>
+srw_tac [][rangevars_def] >- (
+  Cases_on `FLOOKUP s v` >>
+  full_simp_tac (srw_ss()) [FLOOKUP_DEF,FRANGE_DEF] >>
+  metis_tac [] ) >>
+full_simp_tac (srw_ss()) [MEM_MAP,EVERY_MEM,FRANGE_DEF] >>
+metis_tac []);
+
+val NOTIN_FDOM_IN_vars = Q.store_thm(
+"NOTIN_FDOM_IN_vars",
+`!t v s. v IN vars t /\ v NOTIN FDOM s ==> v IN vars (SAPPLY s t)`,
+ho_match_mp_tac term_ind >>
+srw_tac [][] >- (
+  Cases_on `FLOOKUP s v` >>
+  full_simp_tac (srw_ss()) [FLOOKUP_DEF] ) >>
+full_simp_tac (srw_ss()) [MEM_MAP,EVERY_MEM] >>
+metis_tac []);
+
+val IN_FDOM_NOTIN_rangevars = Q.store_thm(
+"IN_FDOM_NOTIN_rangevars",
+`!t v s. v IN FDOM s /\ v NOTIN rangevars s ==> v NOTIN vars (SAPPLY s t)`,
+ho_match_mp_tac term_ind >>
+srw_tac [][rangevars_def] >- (
+  Cases_on `FLOOKUP s v` >>
+  full_simp_tac (srw_ss()) [FLOOKUP_DEF,FRANGE_DEF] >>
+  metis_tac [] ) >>
+full_simp_tac (srw_ss()) [MEM_MAP,EVERY_MEM,FRANGE_DEF] >>
+metis_tac []);
+
+val _ = export_theory ();
